Finish normalization correctness proof

src/tactic/fol/mat.lean
@@ -1,361 +1,149 @@
-import .swap tactic.interactive
+import .folize .list
+
 universe u
 
-variables {α β : Type u}
+variable {α : Type u}
 
-open nat
+open list
 
-local notation f `₀↦` a := assign a f
-postfix  `ₑ` : 1000 := evaluate
-postfix  `ᵈ` : 1000 := denote
-local infix `⬝` := value.app
+local notation `&₁`     := term.sym
+local notation a `&₁` b := term.app a b
+local notation a `#₁` k := term.vpp a k
 
-namespace fol
-
-@[derive has_reflect, derive decidable_eq]
-inductive term : Type
-| sym : nat  → term
-| app : term → term → term
-| vpp : term → nat  → term
-
-inductive form : Type
-| lit : bool → term → form
-| bin : bool → form → form → form
-
-def term.val (M : model α) (v : nat → α) : term → value α
-| (term.sym k)   := M k
-| (term.app a b) := a.val ∘ list.cons (b.val []).fst
-| (term.vpp a k) := a.val ∘ list.cons (v k)
-
-def form.holds (M : model α) (v : nat → α) : form → Prop
-| (form.lit tt a)   :=   (a.val M v []).snd
-| (form.lit ff a)   := ¬ (a.val M v []).snd
-| (form.bin tt p q) := p.holds ∨ q.holds
-| (form.bin ff p q) := p.holds ∧ q.holds
-
-lemma holds_bin_iff_holds_bin
-  {M N : model α} {v w : nat → α} {p q r s : form} {b : bool} :
-  (p.holds M v ↔ q.holds N w) →
-  (r.holds M v ↔ s.holds N w) →
-  ((form.bin b p r).holds M v ↔ (form.bin b q s).holds N w) := sorry
-
-end fol
-
-section
-
-def fam_exv (α : Type u) (p : fol.form) : Prop :=
-∀ M : model α, ∃ v : nat → α, p.holds M v
-
-local notation `&`     := fol.term.sym
-local notation a `&` b := fol.term.app a b
-local notation a `#` k := fol.term.vpp a k
-
-local notation `⟪` b `,` a `⟫` := fol.form.lit b a
-local notation p `∨*` q        := fol.form.bin tt p q
-local notation p `∧*` q        := fol.form.bin ff p q
-
-def term.folize (k : nat) : term → fol.term
-| (term.var m) := (& (m - k))
-| (term.app a (term.var m)) :=
-  if m < k
-  then a.folize # m
-  else a.folize & (& (m - k))
-| (term.app a (term.app b c)) :=
-  a.folize & (term.app b c).folize
-
-def form.folize : nat → form → fol.form
-| k (form.lit b t)   := ⟪b, t.folize k⟫
-| k (form.bin b p q) := fol.form.bin b (p.folize k) (q.folize k)
-| k (form.qua tt p)  := p.folize k.succ
-| k (form.qua ff p)  := p.folize k
-
-def term.fov_lt (k : nat) (a : term) : Prop :=
-∀ m < k, a.fov m
-
-
-lemma fov_lt_of_fov_lt_app_left {k : nat} {a b : term} :
-  (term.app a b).fov_lt k → a.fov_lt k :=
-λ h0 m h1, (h0 m h1).left
-
-lemma fov_lt_of_fov_lt_app_right {k : nat} {a b c : term} :
-  (term.app a (term.app b c)).fov_lt k → (term.app b c).fov_lt k :=
-λ h0 m h1, (h0 m h1).right
-
-def form.fov_lt (k : nat) (p : form) : Prop :=
-∀ m < k, p.fov m
-
-lemma fov_lt_of_fov_lt_bin_left {b : bool} {k : nat} {p q : form} :
-  (form.bin b p q).fov_lt k → p.fov_lt k :=
-λ h0 m h1, (h0 m h1).left
-
-lemma fov_lt_of_fov_lt_bin_right {b : bool} {k : nat} {p q : form} :
-  (form.bin b p q).fov_lt k → q.fov_lt k :=
-λ h0 m h1, (h0 m h1).right
-
-def exs : nat → form → form
-| 0       p := p
-| (k + 1) p := form.qua tt (exs k p)
-
-lemma exs_ex :
-  ∀ k : nat, ∀ p : form,
-  exs k (form.qua tt p) = exs (k + 1) p
-| 0       p := rfl
-| (k + 1) p := by {unfold exs, rw exs_ex, refl}
-
--- lemma fov_exs :
---   ∀ {k m : nat} {p : form}, fov k (exs m p) → fov (k + m) p
--- | k 0       p h0 := h0
--- | k (m + 1) p h0 :=
---   by { convert (@fov_exs (k + 1) m _ h0) using 1,
---        simp only [add_comm,  add_left_comm] }
--- lemma exists_exs :
---   ∀ {p : form}, foq tt p → is_E p →
---   ∃ k : nat, ∃ q : form,
---     (fov_lt k q ∧ is_QF q ∧ p = exs k q)
--- | (form.lit b a)   h0 h1 := ⟨0, (form.lit b a),   trivial, h1, rfl⟩
--- | (form.bin b p q) h0 h1 := ⟨0, (form.bin b p q), trivial, h1, rfl⟩
--- | (form.qua tt p)  h0 h1 :=
---   begin
---     rcases exists_exs h0.right h1 with ⟨k, q, h2, h3, h4⟩,
---     refine ⟨k.succ, q, ⟨_, h2⟩, h3, _⟩,
---     { convert @fov_exs 0 k q _,
---       { rw zero_add },
---       rw ← h4, exact h0.left rfl },
---     congr'
---   end
--- | (form.qua ff p)  h0 h1 := by cases h1
---
-
---lemma holds_of_exv_folize :
---  ∀ {k : nat} {p : form} {M : model α},
---  is_QF p → fov_lt k p →
---  (∃ v : nat → α, (p.folize k).holds M v) →
---  (holds M $ exs k p)
-
-lemma sub_eq_succ_sub_succ {k m : nat} :
-  k + 1 ≤ m → m - k = succ (m - (k + 1)) :=
-begin
-  intro h0,
-  rw succ_le_iff at h0,
-  rw [← nat.sub_sub, ← pred_eq_sub_one, succ_pred_eq_of_pos _],
-  simpa only [gt, nat.lt_sub_left_iff_add_lt] using h0
-end
-
-lemma val_folize_succ {k : nat} (M : model α) (v : nat → α) :
-  ∀ {a : term}, a.fov_lt (k + 1) →
-  (a.folize $ k + 1).val M v = (a.folize k).val (M ₀↦ (v k)ₑ) v
-| (term.var m) h0 :=
-  begin
-    by_cases h1 : m < k + 1,
-    { cases h0 m h1 rfl },
-    rw not_lt at h1,
-    simp only [term.folize, fol.term.val],
-    rw sub_eq_succ_sub_succ h1, refl,
-  end
-| (term.app a (term.var m)) h0 :=
-  begin
-    have h := val_folize_succ (fov_lt_of_fov_lt_app_left h0),
-    unfold term.folize,
-    by_cases h1 : m < k,
-    { rw if_pos h1,
-      rw if_pos (lt_trans h1 $ lt_succ_self _),
-      unfold fol.term.val, rw h },
-    rw if_neg h1,
-    rw not_lt at h1,
-    by_cases h2 : m = k,
-    { rw h2, rw if_pos (lt_succ_self _),
-      unfold fol.term.val,
-      rw [h, nat.sub_self k], refl },
-    have h3 : k + 1 ≤ m,
-    { rw le_iff_eq_or_lt at h1,
-      cases h1,
-      { cases h2 h1.symm },
-      rw succ_le_iff, exact h1 },
-    rw if_neg (not_lt.elim_right h3),
-    unfold fol.term.val,
-    rw [h, sub_eq_succ_sub_succ h3], refl
-  end
-| (term.app a (term.app b c)) h0 :=
-  by simp only [term.folize, fol.term.val,
-     val_folize_succ (fov_lt_of_fov_lt_app_left h0),
-     val_folize_succ (fov_lt_of_fov_lt_app_right h0)]
-
-lemma holds_folize_succ {k : nat} (M : model α) (v : nat → α) :
-  ∀ p : form, is_QF p → p.fov_lt (k + 1) →
-  ((p.folize $ k + 1).holds M v ↔ (p.folize k).holds (M ₀↦ (v k)ₑ) v)
-| (form.lit b a) h0 h1 :=
-  by { cases b; --;
-       simp only  [form.folize, fol.term.val,
-         fol.form.holds, val_folize_succ M v h1] }
-| (form.bin b p q) h0 h1 :=
-  begin
-    apply fol.holds_bin_iff_holds_bin,
-    { exact holds_folize_succ _ h0.left (fov_lt_of_fov_lt_bin_left h1) },
-    exact holds_folize_succ _ h0.right (fov_lt_of_fov_lt_bin_right h1),
-  end
-
-lemma forall_lt_of_forall_lt_succ {k : nat} {p : nat → Prop} :
-  (∀ m < (k + 1), p m) → (∀ m < k, p m) :=
-λ h0 m h1, h0 _ (lt_trans h1 $ lt_succ_self _)
-
-lemma forall_lt_zero {p : nat → Prop} : (∀ m < 0, p m) :=
-λ m h, by cases h
-
-lemma val_folize_zero (M : model α) (v : nat → α) :
-  ∀ a : term, (a.folize 0).val M v = a.val M
-| (term.var k) := rfl
-| (term.app a (term.var k)) :=
-  begin
-    unfold term.folize,
-    have h0 : ¬ k < 0,
-    { rw not_lt, apply nat.zero_le },
-    rw if_neg h0,
-    simp only [fol.term.val, term.val, nat.sub_zero,
-      val_folize_zero a, eq_self_iff_true]
-  end
-| (term.app a (term.app b c)) :=
-  by simp only [fol.term.val, term.val, nat.sub_zero,
-    val_folize_zero a, val_folize_zero (term.app b c),
-    eq_self_iff_true, term.folize]
-
-lemma holds_folize_zero (M : model α) (v : nat → α) :
-  ∀ {p : form}, is_QF p → ((p.folize 0).holds M v ↔ holds M p)
-| (form.lit b a) h0 :=
-  by cases b;
-     simp only [holds, fol.form.holds,
-       form.folize, val_folize_zero]
-| (form.bin b p q) h0 :=
-  by { cases b; apply pred_mono_2;
-       simp only [ holds, fol.form.holds, form.folize,
-       holds_folize_zero h0.left,
-       holds_folize_zero h0.right ] }
-
-
-lemma holds_of_exv_folize :
-  ∀ {p : form} {k : nat} {M : model α},
-  foq tt p → is_E p → p.fov_lt k →
-  (∃ v : nat → α, (p.folize k).holds M v) →
-  (holds M $ exs k p)
-| (form.lit b a) 0  :=
-  by { intros M h0 h1 h2 h3,
-       cases h3 with v h3,
-       rwa holds_folize_zero _ _ h1 at h3 }
-| (form.lit b a) (k + 1) :=
-  begin
-    intros M h0 h1 h2 h3,
-    cases h3 with v h3,
-    rw holds_folize_succ _ _ (form.lit b a) trivial h2 at h3,
-    have h5 : (M ₀↦v k ₑ) ⊨exs k (form.lit b a) :=
-      @holds_of_exv_folize (form.lit b a) k _ trivial
-        trivial (forall_lt_of_forall_lt_succ h2) ⟨v, h3⟩,
-    refine ⟨(v k)ₑ, h5⟩
-  end
-| (form.bin b p q) 0 :=
-  by { intros M h0 h1 h2 h3,
-       cases h3 with v h3,
-       rwa holds_folize_zero _ _ h1 at h3 }
-| (form.bin b p q) (k + 1) :=
-  begin
-intros M h0 h1 h2 h3,
-    cases h3 with v h3,
-    rw holds_folize_succ _ _ (form.bin b p q) h1 h2 at h3,
-    have h5 : (M ₀↦v k ₑ) ⊨exs k (form.bin b p q) :=
-      @holds_of_exv_folize (form.bin b p q) k _ h0
-        h1 (forall_lt_of_forall_lt_succ h2) ⟨v, h3⟩,
-    refine ⟨(v k)ₑ, h5⟩,
-  end
-| (form.qua tt p) k :=
-  begin
-    intros M h0 h1 h2 h3,
-    have h5 : p.fov_lt (k + 1),
-    { rintro ⟨m⟩; intro h4,
-      { exact h0.left rfl },
-      rw succ_lt_succ_iff at h4,
-      exact h2 _ h4 },
-    rw exs_ex,
-    exact @holds_of_exv_folize p (k + 1) M h0.right h1 h5 h3,
-  end
-| (form.qua ff p) k := λ _ _  h, by cases h
-
-lemma fam_of_fam_exv_folize_zero :
-  ∀ {p : form}, foq tt p → is_E p → fam_exv α (p.folize 0) → fam α p :=
-λ p h0 h1 h2 M, @holds_of_exv_folize α p 0 M h0 h1 forall_lt_zero (h2 M)
-
-lemma fam_of_fam_exv_folize :
-  ∀ p : form, foq tt p → is_AE p →
-  fam_exv α (p.folize 0) → fam α p
-| (form.lit b a)   := fam_of_fam_exv_folize_zero
-| (form.bin b p q) := fam_of_fam_exv_folize_zero
-| (form.qua tt p)  := fam_of_fam_exv_folize_zero
-| (form.qua ff p)  :=
-  λ h0 h1 h2, (fam_fa _ _).elim_right
-    (fam_of_fam_exv_folize p h0.right h1 h2)
-
-
-#exit
-
+local notation `⟪` b `,` a `⟫₁` := form.lit b a
+local notation p `∨₁` q        := form.bin tt p q
+local notation p `∧₁` q        := form.bin ff p q
 
 @[reducible] def lit : Type := bool × term
 @[reducible] def cla : Type := list lit
 @[reducible] def mat : Type := list cla
 
-def lit.holds (M : model α) (v : nat → α) : lit → Prop
+namespace lit
+
+def neg : lit → lit
+| ⟨b, a⟩ := ⟨bnot b, a⟩
+
+def repr : lit → string
+| ⟨b, a⟩ := (if b then "" else "¬") ++ a.repr
+
+instance has_repr : has_repr lit := ⟨repr⟩
+
+meta instance has_to_format : has_to_format lit := ⟨λ x, repr x⟩
+
+def vdxs : lit → list nat
+| ⟨b, a⟩ := a.vdxs
+
+def holds (M : model α) (v : nat → α) : lit → Prop
 | (tt, a)  :=    (a.val M v []).snd
 | (ff, a)  :=  ¬ (a.val M v []).snd
 
-def cla.holds (M : model α) (v : nat → α) (c : cla) : Prop :=
+def subst (σ : sub) : lit → lit
+| (b, a) := (b, a.subst σ)
+
+lemma holds_neg (M : model α) (v : nat → α) (l : lit) :
+  holds M v l.neg ↔ ¬ holds M v l :=
+by { cases l with b; cases b; simp only
+     [bnot, neg, holds, list.map, classical.not_not] }
+
+lemma holds_subst (M : model α) (v : vas α) (σ : sub) (l : lit) :
+  holds M v (l.subst σ) ↔ holds M (v.subst M σ) l :=
+by { cases l with b a, cases b;
+     simp only [holds, subst, vas.subst,
+     list.map_map, term.val_subst] }
+
+end lit
+
+namespace cla
+
+def is_pos (C : cla) : bool := C.all prod.fst
+
+def vdxs (C : cla) : list nat := ⋃ (C.map lit.vdxs)
+
+def subst : sub → cla → cla :=
+list.map ∘ lit.subst
+
+def holds (M : model α) (v : nat → α) (c : cla) : Prop :=
 ∀ l ∈ c, lit.holds M v l
 
-def mat.holds (M : model α) (v : nat → α) (m : mat) : Prop :=
+lemma holds_subst {M : model α} {v : vas α} {σ : sub} {c : cla} :
+  holds M v (c.subst σ) ↔ holds M (v.subst M σ) c :=
+begin
+  constructor; intros h1 l h2,
+  { rw ← lit.holds_subst, apply h1,
+    apply list.mem_map_of_mem _ h2 },
+  { have h3 : ∃ x, x ∈ c ∧ lit.subst σ x = l,
+    { rw ← list.mem_map, exact h2 },
+    rcases h3 with ⟨x, h3, h4⟩,
+    rw [←h4, lit.holds_subst],
+    apply h1 _ h3 }
+end
+
+end cla
+
+namespace mat
+
+def holds (M : model α) (v : nat → α) (m : mat) : Prop :=
 ∃ c ∈ m, cla.holds M v c
+
+lemma holds_cons {M : model α} {v : nat → α} (c : cla) (m : mat) :
+mat.holds M v (c :: m) ↔ (c.holds M v ∨ m.holds M v) :=
+by simp only [mat.holds, list.exists_mem_cons_iff]
 
 def fam_exv (α : Type u) (m : mat) : Prop :=
 ∀ M : model α, ∃ v : nat → α, m.holds M v
 
+end mat
 
+def dnf : form → mat
+| ⟪b, a⟫₁   := [[(b, a)]]
+| (p ∧₁ q) := (list.product (dnf p) (dnf q)).map (λ x, x.fst ++ x.snd)
+| (p ∨₁ q) := (dnf p) ++ (dnf q)
 
-
-#exit
-def dnf : nat → form → mat
-| k ⟪b, a⟫   := [[(b, symbolize k a)]]
-| k (p ∨* q) := dnf k p ++ dnf k q
-| k (p ∧* q) :=
-  (list.product (dnf k p) (dnf k q)).map (λ x, x.fst ++ x.snd)
-| k (∀* p)   := dnf k p
-| k (∃* p)   := dnf k.succ p
-
-lemma fam_exv_dnf :
-  ∀ k : nat, ∀ p : form, is_E p →
-  (fam_exv α (dnf k p) ↔ fam α p)
-| k (∃* p) h0 :=
+lemma holds_of_holds_dnf {M : model α} {v : nat → α} :
+  ∀ p : form, (dnf p).holds M v → p.holds M v
+| ⟪b, a⟫₁ h0 :=
   begin
-    simp only [dnf],
-    have h1 := fam_exv_dnf k.succ p h0,
-
+    rcases h0 with ⟨c, h3, h4⟩,
+    rw eq_of_mem_singleton h3 at h4,
+    cases b; exact h4 _ (or.inl rfl)
+  end
+| (p ∨₁ q) h0 :=
+  begin
+    rcases h0 with ⟨c, h3, h4⟩,
+    cases mem_append.elim_left h3 with h5 h5,
+    apply or.inl (holds_of_holds_dnf _ ⟨c, h5, h4⟩),
+    apply or.inr (holds_of_holds_dnf _ ⟨c, h5, h4⟩)
+  end
+| (p ∧₁ q) h0 :=
+  begin
+    rcases h0 with ⟨c, h3, h4⟩,
+    rcases mem_map.elim_left h3 with ⟨⟨_, _⟩, h5, h6⟩,
+    cases mem_product.elim_left h5 with hl hr,
+    rw ← h6 at h4,
+    cases forall_mem_append.elim_left h4,
+    refine ⟨ holds_of_holds_dnf _ ⟨_, hl, _⟩,
+             holds_of_holds_dnf _ ⟨_, hr, _⟩ ⟩;
+    assumption,
   end
 
+lemma fam_exv_of_dnf_fam_exv {p : form} :
+  (dnf p).fam_exv α → p.fam_exv α :=
+by { intros h1 M, cases h1 M with v h1,
+     refine ⟨v, holds_of_holds_dnf p h1⟩ }
 
-#exit
-lemma fam_exv_dnf_zero :
-  ∀ p : form, is_AE p →
-  (fam_exv α (dnf 0 p) ↔ fam α p)
-| (∀* p) h0 :=
-  iff.trans
-    (fam_exv_dnf_zero p h0)
-    (fam_fa _ _).symm
-| (∃* p)           h0 := fam_exv_dnf 0 _ h0
-| (form.bin b p q) h0 := fam_exv_dnf 0 _ h0
-| ⟪b, a⟫           h0 := fam_exv_dnf 0 _ h0
+def normalize : form₂ → mat :=
+dnf ∘ form₂.folize 0 ∘ QDFy ff
 
-
-#exit
-
-def mix (M N : model α) (k : nat) : model α :=
-λ m, if m < k then M k else N k
-
-def lit.holds (M N : model α) (k : nat) : lit → Prop
-| (tt, a) :=   (a.val (mix M N k) []).snd
-| (ff, a) := ¬ (a.val (mix M N k) []).snd
-
-
-#exit
+lemma holds_of_fam_exv_normalize
+  [inhabited α] (p : form₂)  :
+  foq tt p → (normalize p).fam_exv α → holds (model.default α) p :=
+begin
+  intros h0 h1,
+  have h2 := fam_exv_of_dnf_fam_exv h1,
+  have h3 := fam_of_fam_exv_folize _
+    (foq_prenexify _ $ foq_swap_all _ h0)
+    (QDF_QDFy _ _) h2 (model.default α),
+  rwa [prenexify_eqv _ (model.default α),
+      swap_all_eqv _ (model.default α)] at h3,
+  apply h0,
+end
