src/tactic/fol/model.lean
@@ -1,6 +1,6 @@
-import  .misc logic.function
+import .misc logic.function
 
-universe u 
+universe u
 
 variable {α : Type u}
 
@@ -8,7 +8,7 @@ local notation f `₀↦` a := assign a f
 
 def value (α : Type u) : Type u := list α → (α × Prop)
 
-def value.default [inhabited α] : value α := 
+def value.default [inhabited α] : value α :=
 λ as, (default α, false)
 
 def evaluate (a : α) : value α :=
@@ -16,22 +16,27 @@ def evaluate (a : α) : value α :=
 
 def denote (v : value α) : α := (v []).fst
 
-postfix  `ₑ` : 1000 := evaluate 
+postfix  `ₑ` : 1000 := evaluate
 postfix  `ᵈ` : 1000 := denote
 
 lemma denote_evaluate (a : α) : (a ₑ)ᵈ = a := rfl
 
-@[reducible] def value.app (v w : value α) : value α := 
+@[reducible] def value.app (v w : value α) : value α :=
 λ as, v (wᵈ :: as)
 
 local infix `⬝` := value.app
+
 def model (α : Type u) : Type u := nat → value α
 
+def model.default (α : Type u) [inhabited α] : model α := λ _, value.default
+
+@[reducible] def vas (α : Type u) : Type u := nat → α
+
 lemma assign_app_evaluate_denote (M : model α) (v w : value α) :
-  (M ₀↦ v ⬝ wᵈₑ) = (M ₀↦ v ⬝ w) := 
+  (M ₀↦ v ⬝ wᵈₑ) = (M ₀↦ v ⬝ w) :=
 by ext k as; cases k; refl
 
-namespace model 
+namespace model
 
 def decr_idxs (M : model α) : model α :=
 M ∘ nat.succ
@@ -39,7 +44,7 @@ M ∘ nat.succ
 end model
 
 lemma assign_decr_idxs (M : model α) :
-  (M.decr_idxs ₀↦ (M 0)) = M := 
+  (M.decr_idxs ₀↦ (M 0)) = M :=
 begin
   rw function.funext_iff,
   rintro ⟨_⟩, { refl },
