src/tactic/fol/pull.lean
@@ -7,116 +7,116 @@ variables {α β : Type u}
 open nat
 
 local notation f `₀↦` a := assign a f
-local notation `#` := term.var
-local notation a `&` b := term.app a b
+local notation `#` := term₂.var
+local notation a `&` b := term₂.app a b
 
 postfix  `ₑ` : 1000 := evaluate
 postfix  `ᵈ` : 1000 := denote
 local infix `⬝` := value.app
 
-local notation `⟪` b `,` a `⟫` := form.lit b a
-local notation p `∨*` q        := form.bin tt p q
-local notation p `∧*` q        := form.bin ff p q
-local notation `∃*`            := form.qua tt
-local notation `∀*`            := form.qua ff
+local notation `⟪` b `,` a `⟫` := form₂.lit b a
+local notation p `∨*` q        := form₂.bin tt p q
+local notation p `∧*` q        := form₂.bin ff p q
+local notation `∃*`            := form₂.qua tt
+local notation `∀*`            := form₂.qua ff
 
-def pull_fa_left_eqv [inhabited α] (b : bool) (p q : form) :
-  ∀* (form.bin b p q.incr_idxs) <==α==> form.bin b (∀* p) q :=
+def pull_fa_left_eqv [inhabited α] (b : bool) (p q : form₂) :
+  ∀* (form₂.bin b p q.incr) <==α==> form₂.bin b (∀* p) q :=
 begin
   intro M,
   have v : value α := (default α)ₑ,
   constructor; intro h0; cases b,
   { constructor,
     { intro w, exact (h0 w).left },
-    apply (holds_assign_incr_idxs _).elim_left (h0 v).right },
-  { cases classical.em ((M ₀↦ v) ⊨ q.incr_idxs) with h2 h2,
-    { rw holds_assign_incr_idxs at h2,
+    apply (holds_assign_incr _).elim_left (h0 v).right },
+  { cases classical.em ((M ₀↦ v) ⊨ q.incr) with h2 h2,
+    { rw holds_assign_incr at h2,
       right, exact h2 },
     left, intro w,
     cases (h0 w) with h3 h3,
     { exact h3 },
-    rw holds_assign_incr_idxs at h2,
-    rw holds_assign_incr_idxs at h3,
+    rw holds_assign_incr at h2,
+    rw holds_assign_incr at h3,
     cases (h2 h3) },
   { intro w,
     refine ⟨h0.left _, _⟩,
-    rw holds_assign_incr_idxs,
+    rw holds_assign_incr,
     exact h0.right },
   { intro w,
-    cases classical.em ((M ₀↦ w) ⊨ q.incr_idxs) with h1 h1,
+    cases classical.em ((M ₀↦ w) ⊨ q.incr) with h1 h1,
     { right, exact h1 },
     left, cases h0 with h2 h2,
     { apply h2 },
-    rw holds_assign_incr_idxs at h1,
+    rw holds_assign_incr at h1,
     cases (h1 h2) }
 end
 
-def pull_ex_left_eqv [inhabited α] (b : bool) (p q : form) :
-  ∃* (form.bin b p q.incr_idxs) <==α==> form.bin b (∃* p) q :=
+def pull_ex_left_eqv [inhabited α] (b : bool) (p q : form₂) :
+  ∃* (form₂.bin b p q.incr) <==α==> form₂.bin b (∃* p) q :=
 by { rw ← neg_eqv_neg,
-     simp only [form.neg, neg_incr_idxs,
+     simp only [form₂.neg, neg_incr,
      bnot, pull_fa_left_eqv] }
 
 
-def pull_left_eqv [inhabited α] (ae ao : bool) (p q : form) :
-  form.qua ae (form.bin ao p q.incr_idxs) <==α==>
-  form.bin ao (form.qua ae p) q :=
+def pull_left_eqv [inhabited α] (ae ao : bool) (p q : form₂) :
+  form₂.qua ae (form₂.bin ao p q.incr) <==α==>
+  form₂.bin ao (form₂.qua ae p) q :=
 by {cases ae, apply pull_fa_left_eqv, apply pull_ex_left_eqv }
 
--- def pull_right_eqv [inhabited α] (ae ao : bool) (p q : form) :
---   form.qua ae (form.bin ao p.incr_idxs q) <==α==>
---   form.bin ao p (form.qua ae q) :=
+-- def pull_right_eqv [inhabited α] (ae ao : bool) (p q : form₂) :
+--   form₂.qua ae (form₂.bin ao p.incr q) <==α==>
+--   form₂.bin ao p (form₂.qua ae q) :=
 -- begin
---   have h0 : ( form.qua ae (form.bin ao (form.incr_idxs p) q) <==α==>
---               form.qua ae (form.bin ao q (form.incr_idxs p)) ) :=
+--   have h0 : ( form₂.qua ae (form₂.bin ao (form₂.incr p) q) <==α==>
+--               form₂.qua ae (form₂.bin ao q (form₂.incr p)) ) :=
 --   qua_eqv_qua (bin_comm _ _ _),
 --   intro M,
 --   simp only [ h0 M, pull_left_eqv ae ao q p M,
---     bin_comm ao p (form.qua ae q) M ]
+--     bin_comm ao p (form₂.qua ae q) M ]
 -- end
 
-@[reducible] def form.size_of_ordered :
-  (Σ' (b : bool), (Σ' (a : form), form)) → nat
+@[reducible] def form₂.size_of_ordered :
+  (Σ' (b : bool), (Σ' (a : form₂), form₂)) → nat
 | ⟨tt, p, q⟩ := p.size_of + q.size_of + 1
 | ⟨ff, p, q⟩ := p.size_of + q.size_of
 
-meta def form.show_size_lt : tactic unit :=
-`[ simp only [form.size_of_ordered, form.size_of,
+meta def form₂.show_size_lt : tactic unit :=
+`[ simp only [form₂.size_of_ordered, form₂.size_of,
    nat.lt_succ_self, add_comm, add_lt_add_iff_left,
-   add_left_comm, form.size_of_incr_idxs ] ]
+   add_left_comm, form₂.size_of_incr ] ]
 
 /- Pull quantifiers over a binary connective. `ae` specifies
    the type of quantifier to be pulled, and `ao` specifies
    the binary connective. -/
-def pull (ae : option bool) (ao : bool) : bool → form → form → form
-| tt (form.qua b p) q :=
-  have form.size_of_ordered ⟨ff, ⟨q, form.qua b p⟩⟩ <
-       form.size_of_ordered ⟨tt, ⟨form.qua b p, q⟩⟩,
-  by form.show_size_lt,
+def pull (ae : option bool) (ao : bool) : bool → form₂ → form₂ → form₂
+| tt (form₂.qua b p) q :=
+  have form₂.size_of_ordered ⟨ff, ⟨q, form₂.qua b p⟩⟩ <
+       form₂.size_of_ordered ⟨tt, ⟨form₂.qua b p, q⟩⟩,
+  by form₂.show_size_lt,
   if ae = some (bnot b)
-  then pull ff q (form.qua b p)
-  else form.qua b (pull tt p q.incr_idxs)
-| ff (form.qua b p) q :=
-  have form.size_of_ordered ⟨ff, ⟨p, form.incr_idxs q⟩⟩ <
-       form.size_of_ordered ⟨ff, ⟨form.qua b p, q⟩⟩,
-  by form.show_size_lt,
+  then pull ff q (form₂.qua b p)
+  else form₂.qua b (pull tt p q.incr)
+| ff (form₂.qua b p) q :=
+  have form₂.size_of_ordered ⟨ff, ⟨p, form₂.incr q⟩⟩ <
+       form₂.size_of_ordered ⟨ff, ⟨form₂.qua b p, q⟩⟩,
+  by form₂.show_size_lt,
   if ae = some (bnot b)
-  then form.bin ao (form.qua b p) q
-  else form.qua b (pull ff p q.incr_idxs)
+  then form₂.bin ao (form₂.qua b p) q
+  else form₂.qua b (pull ff p q.incr)
 | tt p q :=
-  have form.size_of_ordered ⟨ff, ⟨q, p⟩⟩ <
-       form.size_of_ordered ⟨tt, ⟨p, q⟩⟩,
-  by form.show_size_lt,
+  have form₂.size_of_ordered ⟨ff, ⟨q, p⟩⟩ <
+       form₂.size_of_ordered ⟨tt, ⟨p, q⟩⟩,
+  by form₂.show_size_lt,
   pull ff q p
-| ff p q := form.bin ao p q
+| ff p q := form₂.bin ao p q
 using_well_founded
-  {rel_tac := λ _ _, `[exact ⟨_, measure_wf form.size_of_ordered⟩]}
+  {rel_tac := λ _ _, `[exact ⟨_, measure_wf form₂.size_of_ordered⟩]}
 
 lemma fov_pull (ae : option bool) (ao : bool) :
-  ∀ (ls : bool) {p q : form} {k : nat},
+  ∀ (ls : bool) {p q : form₂} {k : nat},
   p.fov k → q.fov k → (pull ae ao ls p q).fov k
 | tt ⟪m, a⟫           q :=
-  have 0 < form.size_of ⟪m,a⟫ := zero_lt_one,
+  have 0 < form₂.size_of ⟪m,a⟫ := zero_lt_one,
   by { intros k h0 h1,
        unfold pull,
        apply fov_pull ff h1 h0 }
@@ -124,21 +124,21 @@ lemma fov_pull (ae : option bool) (ao : bool) :
   by { intros k h0 h1,
        unfold pull,
        refine ⟨h0, h1⟩ }
-| tt (form.bin b p q) r :=
-  have form.size_of_ordered ⟨ff, ⟨r, form.bin b p q⟩⟩ <
-       form.size_of_ordered ⟨tt, ⟨form.bin b p q, r⟩⟩,
-  by form.show_size_lt,
+| tt (form₂.bin b p q) r :=
+  have form₂.size_of_ordered ⟨ff, ⟨r, form₂.bin b p q⟩⟩ <
+       form₂.size_of_ordered ⟨tt, ⟨form₂.bin b p q, r⟩⟩,
+  by form₂.show_size_lt,
   by { intros k h0 h1,
        unfold pull,
        apply fov_pull ff h1 h0 }
-| ff (form.bin b p q) r :=
+| ff (form₂.bin b p q) r :=
   by { intros k h0 h1,
        unfold pull,
        refine ⟨h0, h1⟩ }
-| tt (form.qua b p)   q :=
-  have form.size_of_ordered ⟨ff, ⟨q, form.qua b p⟩⟩ <
-       form.size_of_ordered ⟨tt, ⟨form.qua b p, q⟩⟩,
-  by form.show_size_lt,
+| tt (form₂.qua b p)   q :=
+  have form₂.size_of_ordered ⟨ff, ⟨q, form₂.qua b p⟩⟩ <
+       form₂.size_of_ordered ⟨tt, ⟨form₂.qua b p, q⟩⟩,
+  by form₂.show_size_lt,
   begin
     intros k h0 h1,
     unfold pull,
@@ -146,12 +146,12 @@ lemma fov_pull (ae : option bool) (ao : bool) :
     { apply fov_pull ff h1 h0 },
     apply fov_pull,
     { apply h0 },
-    apply fov_incr_idxs h1
+    apply fov_incr h1
   end
-| ff (form.qua b p)   q :=
-  have form.size_of_ordered ⟨ff, ⟨p, form.incr_idxs q⟩⟩ <
-       form.size_of_ordered ⟨ff, ⟨form.qua b p, q⟩⟩,
-  by form.show_size_lt,
+| ff (form₂.qua b p)   q :=
+  have form₂.size_of_ordered ⟨ff, ⟨p, form₂.incr q⟩⟩ <
+       form₂.size_of_ordered ⟨ff, ⟨form₂.qua b p, q⟩⟩,
+  by form₂.show_size_lt,
   begin
     intros k h0 h1,
     unfold pull,
@@ -159,52 +159,189 @@ lemma fov_pull (ae : option bool) (ao : bool) :
     { refine ⟨h0, h1⟩ },
     apply fov_pull,
     { apply h0 },
-    apply fov_incr_idxs h1
+    apply fov_incr h1
   end
 using_well_founded
-  { rel_tac := λ _ _, `[exact ⟨_, measure_wf form.size_of_ordered⟩] }
+  { rel_tac := λ _ _, `[exact ⟨_, measure_wf form₂.size_of_ordered⟩] }
+
+lemma foq_pull (ae : option bool) (ao b : bool) :
+  ∀ ls : bool, ∀ {p q : form₂},
+  foq b p → foq b q → foq b (pull ae ao ls p q)
+| tt ⟪m, a⟫           q :=
+  have 0 < form₂.size_of ⟪m,a⟫ := zero_lt_one,
+  by { intros h0 h1,
+       unfold pull,
+       apply foq_pull _ h1 h0 }
+| ff ⟪m, a⟫           q :=
+  by { intros h0 h1,
+       unfold pull,
+       refine ⟨h0, h1⟩ }
+| tt (form₂.bin b p q) r :=
+  have form₂.size_of_ordered ⟨ff, ⟨r, form₂.bin b p q⟩⟩ <
+       form₂.size_of_ordered ⟨tt, ⟨form₂.bin b p q, r⟩⟩,
+  by form₂.show_size_lt,
+  by { intros h0 h1,
+       unfold pull,
+       apply foq_pull _ h1 h0 }
+| ff (form₂.bin b p q) r :=
+  by { intros h0 h1,
+       unfold pull,
+       refine ⟨h0, h1⟩ }
+| tt (form₂.qua b p)   q :=
+  have form₂.size_of_ordered ⟨ff, ⟨q, form₂.qua b p⟩⟩ <
+       form₂.size_of_ordered ⟨tt, ⟨form₂.qua b p, q⟩⟩,
+  by form₂.show_size_lt,
+  begin
+    intros h0 h1,
+    unfold pull,
+    apply ite_cases,
+    { apply foq_pull _ h1 h0 },
+    refine ⟨λ h2, _, _⟩,
+    { subst h2,
+      apply fov_pull _ _ _ (h0.left rfl),
+      apply form₂.fov_of_not_occ,
+      apply form₂.not_occ_incr_ge },
+    apply foq_pull _ h0.right,
+    apply foq_incr_ge h1
+  end
+| ff (form₂.qua c p)   q :=
+  have form₂.size_of_ordered ⟨ff, ⟨p, form₂.incr q⟩⟩ <
+       form₂.size_of_ordered ⟨ff, ⟨form₂.qua b p, q⟩⟩,
+  by form₂.show_size_lt,
+  begin
+    intros h0 h1,
+    unfold pull,
+    apply ite_cases,
+    { refine ⟨h0, h1⟩ },
+    refine ⟨λ h2, _, _⟩,
+    { subst h2,
+      apply fov_pull _ _ _ (h0.left rfl),
+      apply form₂.fov_of_not_occ,
+      apply form₂.not_occ_incr_ge },
+    apply foq_pull _ h0.right,
+    apply foq_incr_ge h1
+  end
+using_well_founded
+  { rel_tac := λ _ _, `[exact ⟨_, measure_wf form₂.size_of_ordered⟩] }
 
 def pull_eqv [inhabited α] (ae : option bool) (ao : bool) :
-  ∀ ls : bool, ∀ p q : form,
-  pull ae ao ls p q <==α==> form.bin ao p q
+  ∀ ls : bool, ∀ p q : form₂,
+  pull ae ao ls p q <==α==> form₂.bin ao p q
 | tt ⟪k, a⟫           q :=
-  have 0 < form.size_of ⟪k,a⟫ := zero_lt_succ _,
+  have 0 < form₂.size_of ⟪k,a⟫ := zero_lt_succ _,
   by { apply eqv_trans _ (bin_comm _ _ _),
        unfold pull,
        apply pull_eqv }
 | ff ⟪k, a⟫           q := by {unfold pull, apply eqv_refl}
-| tt (form.bin b p q) r :=
-  have form.size_of_ordered ⟨ff, ⟨r, form.bin b p q⟩⟩ <
-       form.size_of_ordered ⟨tt, ⟨form.bin b p q, r⟩⟩,
-  by form.show_size_lt,
+| tt (form₂.bin b p q) r :=
+  have form₂.size_of_ordered ⟨ff, ⟨r, form₂.bin b p q⟩⟩ <
+       form₂.size_of_ordered ⟨tt, ⟨form₂.bin b p q, r⟩⟩,
+  by form₂.show_size_lt,
   by { apply eqv_trans _ (bin_comm _ _ _),
        unfold pull,
        apply pull_eqv }
-| ff (form.bin b p q) r := by {unfold pull, apply eqv_refl}
-| tt (form.qua b p) q :=
-  have  form.size_of_ordered ⟨ff, ⟨q, form.qua b p⟩⟩ <
-        form.size_of_ordered ⟨tt, ⟨form.qua b p, q⟩⟩,
-  by form.show_size_lt,
+| ff (form₂.bin b p q) r := by {unfold pull, apply eqv_refl}
+| tt (form₂.qua b p) q :=
+  have  form₂.size_of_ordered ⟨ff, ⟨q, form₂.qua b p⟩⟩ <
+        form₂.size_of_ordered ⟨tt, ⟨form₂.qua b p, q⟩⟩,
+  by form₂.show_size_lt,
   begin
     unfold pull,
-    apply @ite_cases _ (λ x, x <==α==>form.bin ao (form.qua b p) q),
+    apply @ite_cases _ (λ x, x <==α==>form₂.bin ao (form₂.qua b p) q),
     { apply eqv_trans _ (bin_comm _ _ _),
       apply pull_eqv },
     apply eqv_trans
       (qua_eqv_qua $ pull_eqv _ p _)
       (pull_left_eqv _ _ _ _)
   end
-| ff (form.qua b p) q :=
-  have  form.size_of_ordered ⟨ff, ⟨p, form.incr_idxs q⟩⟩ <
-        form.size_of_ordered ⟨ff, ⟨form.qua b p, q⟩⟩,
-  by form.show_size_lt,
+| ff (form₂.qua b p) q :=
+  have  form₂.size_of_ordered ⟨ff, ⟨p, form₂.incr q⟩⟩ <
+        form₂.size_of_ordered ⟨ff, ⟨form₂.qua b p, q⟩⟩,
+  by form₂.show_size_lt,
   begin
     unfold pull,
-    apply @ite_cases _ (λ x, x <==α==>form.bin ao (form.qua b p) q),
+    apply @ite_cases _ (λ x, x <==α==>form₂.bin ao (form₂.qua b p) q),
     { apply eqv_refl },
     apply eqv_trans
       (qua_eqv_qua $ pull_eqv _ p _)
       (pull_left_eqv _ _ _ _),
   end
 using_well_founded
-  {rel_tac := λ _ _, `[exact ⟨_, measure_wf form.size_of_ordered⟩]}
+  {rel_tac := λ _ _, `[exact ⟨_, measure_wf form₂.size_of_ordered⟩]}
+
+lemma QN_pull_aux {b : bool} (ao : bool) :
+  ∀ {p q : form₂}, p.QN b → q.N b →
+  (pull (some b) ao ff p q).QN b
+| (form₂.lit c a) q h0 h1 :=
+  by {unfold pull, refine ⟨h0, h1⟩}
+| (form₂.bin c p q) r h0 h1 :=
+  by {unfold pull, refine ⟨h0, h1⟩}
+| (form₂.qua c p) q h0 h1 :=
+  begin
+    unfold pull,
+    by_cases h2 : b = bnot c,
+    { rw [← h2, if_pos rfl],
+      rw eq_bnot_iff_ne at h2,
+      refine ⟨⟨h2, h0.right h2⟩, h1⟩ },
+    rw if_neg,
+    { have h3 : b = c,
+      { rw eq_bnot_iff_ne at h2,
+        apply not_not.elim_left h2 },
+      refine ⟨λ _, _, λ h4, absurd h3 h4⟩,
+      apply QN_pull_aux (h0.left h3),
+      apply form₂.N_incr_ge _ h1 },
+    rw option.some_inj, exact h2
+  end
+
+lemma QN_pull {b : bool} (ao : bool) :
+  ∀ {p q : form₂}, p.QN b → q.QN b →
+  (pull (some b) ao tt p q).QN b
+| (form₂.lit c a) q h0 h1 :=
+  by {unfold pull, apply QN_pull_aux _ h1 h0}
+| (form₂.bin _ p q) r h0 h1 :=
+  by {unfold pull, apply QN_pull_aux _ h1 h0}
+| (form₂.qua c p) q h0 h1 :=
+  begin
+    unfold pull,
+    by_cases h2 : b = bnot c,
+    { rw [← h2, if_pos rfl],
+      rw eq_bnot_iff_ne at h2,
+      apply QN_pull_aux _ h1,
+      refine ⟨h2, h0.right h2⟩ },
+    rw if_neg,
+    { rw [eq_bnot_iff_ne, not_not] at h2,
+      refine ⟨λ _, _, λ h3, absurd h2 h3⟩,
+      apply QN_pull (h0.left h2),
+      apply form₂.QN_incr_ge _ h1 },
+    rw option.some_inj, exact h2
+  end
+
+lemma QF_pull_aux {b : bool} (ao : bool) :
+  ∀ {p q : form₂}, p.QF b → q.F →
+  (pull none ao ff p q).QF b
+| (form₂.lit c a)   q h0 h1 :=
+  by {unfold pull, refine ⟨h0, h1⟩}
+| (form₂.bin c p q) r h0 h1 :=
+  by {unfold pull, refine ⟨h0, h1⟩}
+| (form₂.qua c p) q h0 h1 :=
+  begin
+    unfold pull, rw if_neg,
+    { refine ⟨h0.left,
+        QF_pull_aux h0.right (form₂.F_incr_ge _ h1)⟩ },
+    rintro ⟨_⟩,
+  end
+
+lemma QF_pull {b : bool} (ao : bool) :
+  ∀ {p q : form₂}, p.QF b → q.QF b →
+  (pull none ao tt p q).QF b
+| (form₂.lit c a) q h0 h1 :=
+  by {unfold pull, apply QF_pull_aux _ h1 h0 }
+| (form₂.bin _ p q) r h0 h1 :=
+  by {unfold pull, apply QF_pull_aux _ h1 h0 }
+| (form₂.qua c p) q h0 h1 :=
+  begin
+    unfold pull, rw if_neg,
+    { refine ⟨h0.left,
+        QF_pull h0.right (form₂.QF_incr_ge _ h1)⟩ },
+    intro h2, cases h2
+  end
