src/tactic/fol/swap.lean
@@ -9,20 +9,17 @@ open nat
 local notation f `₀↦` a := assign a f
 local infix `⬝` := value.app
 
-local notation `#` := term.var
-local notation a `&` b := term.app a b
+local notation `#` := term₂.var
+local notation a `&` b := term₂.app a b
 
-local notation `⟪` b `,` a `⟫` := form.lit b a
-local notation p `∨*` q        := form.bin tt p q
-local notation p `∧*` q        := form.bin ff p q
-local notation `∃*`            := form.qua tt
-local notation `∀*`            := form.qua ff
+local notation `⟪` b `,` a `⟫` := form₂.lit b a
+local notation p `∨*` q        := form₂.bin tt p q
+local notation p `∧*` q        := form₂.bin ff p q
+local notation `∃*`            := form₂.qua tt
+local notation `∀*`            := form₂.qua ff
 
-@[reducible] def swap (k : nat) : sub :=
+@[reducible] def swap (k : nat) : sub₂ :=
 [(k, # (k + 1) & # k), (k + 1, # k)]
-
-def form.swap (k : nat) (p : form) : form :=
-p.subst (swap k)
 
 lemma subst_swap_var (k m : nat) :
 (m = k ∧ (# m).subst (swap k) = (# (k + 1) & # k)) ∨
@@ -31,42 +28,44 @@ lemma subst_swap_var (k m : nat) :
 begin
   by_cases h0 : m = k,
   { left, refine ⟨h0, _⟩,
-    simp only [ swap, term.subst, sub.get,
+    simp only [ swap, term₂.subst, sub₂.get,
       if_true, h0, eq_self_iff_true ], refl },
   by_cases h1 : m = k + 1,
   { right, left,
     refine ⟨h1, _⟩,
-    simp only [ swap, term.subst, sub.get,
+    simp only [ swap, term₂.subst, sub₂.get,
       if_neg h0, if_pos h1 ], refl },
   right, right,
   refine ⟨h0, h1, _⟩,
-  simp only [ swap, term.subst, sub.get,
+  simp only [ swap, term₂.subst, sub₂.get,
     if_neg h0, if_neg h1 ], refl
 end
 
-lemma fov_succ_succ (k m : nat) (h0 : m + 1 < k) :
-  ∀ a : term, a.fov k → (a.subst $ swap m).fov k
+namespace term₂
+
+lemma fov_swap_of_ne {k m : nat} (hO : k ≠ m) (hS : k ≠ m + 1) :
+  ∀ a : term₂, a.fov k → (a.subst $ swap m).fov k
 | (# n) h1 :=
   begin
     rcases subst_swap_var m n
       with ⟨_, h2⟩ | ⟨_, h2⟩ | ⟨_, _, h2⟩; rw h2,
-    { refine ⟨ne_of_gt h0, trivial⟩ },
-    { exact ne_of_gt (lt_trans (lt_succ_self _) h0) },
-    exact h1
+    { refine ⟨hS, trivial⟩ },
+    { exact hO },
+    exact h1,
   end
 | (a & (# n)) h1 :=
   begin
-    refine ⟨fov_succ_succ a h1.left, _⟩,
+    refine ⟨fov_swap_of_ne _ h1.left, _⟩,
     rcases subst_swap_var m n
       with ⟨_, h2⟩ | ⟨_, h2⟩ | ⟨_, _, h2⟩;
     rw h2; try {exact trivial},
-    refine ⟨ne_of_gt h0, trivial⟩,
+    refine ⟨hS, trivial⟩
   end
 | (a & (b & c)) h1 :=
-  ⟨fov_succ_succ a h1.left, fov_succ_succ (b &c) h1.right⟩
+  ⟨fov_swap_of_ne _ h1.left, fov_swap_of_ne (b &c) h1.right⟩
 
-lemma fov_succ (k : nat) :
-  ∀ a : term, a.fov (k + 1) → (a.subst $ swap k).fov k
+lemma fov_swap (k : nat) :
+  ∀ a : term₂, a.fov (k + 1) → (a.subst $ swap k).fov k
 | (# m) h0 :=
   begin
     rcases subst_swap_var k m
@@ -78,19 +77,47 @@ lemma fov_succ (k : nat) :
   end
 | (a & (# m)) h0 :=
   begin
-    refine ⟨fov_succ _ h0.left, _⟩,
+    refine ⟨fov_swap _ h0.left, _⟩,
     rcases subst_swap_var k m
       with ⟨_, h1⟩ | ⟨h2, h1⟩ | ⟨h2, _, h1⟩;
     rw h1; try {exact trivial},
     refine ⟨(succ_ne_self _).symm, trivial⟩
   end
 | (a & (b & c)) h0 :=
-  ⟨fov_succ a h0.left, fov_succ (b &c) h0.right⟩
+  ⟨fov_swap a h0.left, fov_swap (b &c) h0.right⟩
 
-lemma holds_swap {M : model α} {v w : value α} {p : form} :
+end term₂
+
+
+def form₂.swap (k : nat) (p : form₂) : form₂ :=
+p.subst (swap k)
+
+-- lemma fov_succ_succ (k m : nat) (h0 : m + 1 < k) :
+--   ∀ a : term₂, a.fov k → (a.subst $ swap m).fov k
+-- | (# n) h1 :=
+--   begin
+--     rcases subst_swap_var m n
+--       with ⟨_, h2⟩ | ⟨_, h2⟩ | ⟨_, _, h2⟩; rw h2,
+--     { refine ⟨ne_of_gt h0, trivial⟩ },
+--     { exact ne_of_gt (lt_trans (lt_succ_self _) h0) },
+--     exact h1
+--   end
+-- | (a & (# n)) h1 :=
+--   begin
+--     refine ⟨fov_succ_succ a h1.left, _⟩,
+--     rcases subst_swap_var m n
+--       with ⟨_, h2⟩ | ⟨_, h2⟩ | ⟨_, _, h2⟩;
+--     rw h2; try {exact trivial},
+--     refine ⟨ne_of_gt h0, trivial⟩,
+--   end
+-- | (a & (b & c)) h1 :=
+--   ⟨fov_succ_succ a h1.left, fov_succ_succ (b &c) h1.right⟩
+
+
+lemma holds_swap {M : model α} {v w : value α} {p : form₂} :
   ((M ₀↦ v ₀↦ w) ⊨ p.swap 0) ↔ ((M ₀↦ w ₀↦ v ⬝ w) ⊨ p) :=
 begin
-  unfold form.swap,
+  unfold form₂.swap,
   rw holds_subst,
   have h0 : model.subst (M ₀↦ v ₀↦ w) [(0, (# 1) & (# 0)), (1, # 0)] =
             (M ₀↦ w ₀↦ v ⬝ w),
@@ -104,7 +131,7 @@ def swap_val [inhabited α] (f : value α → value α) : value α
 | []        := (default α, false)
 | (a :: as) := f (a ₑ) as
 
-lemma exists_swap_val [inhabited α] {M : model α} {p : form} :
+lemma exists_swap_val [inhabited α] {M : model α} {p : form₂} :
   (M ⊨ ∀* (∃* p)) → ∃ f : value α, ∀ a : α, (M ₀↦ (a ₑ) ₀↦ f ⬝ a ₑ) ⊨ p :=
 begin
   intro h0,
@@ -127,18 +154,18 @@ begin
 end
 
 lemma val_eq_val_of_eq_except {M N : model α} {k : nat} (h0 : eq_except M N k) :
-  ∀ a : term, a.fov k → (a.val M = a.val N)
+  ∀ a : term₂, a.fov k → (a.val M = a.val N)
 | (# m)   h1 := by apply h0.left _ (ne.symm h1)
 | (a & (# m)) h1 :=
   begin
     have h2 : a.val M = a.val N,
-    { rw term.fov_app_var at h1,
+    { rw term₂.fov_app_var at h1,
       apply val_eq_val_of_eq_except a h1 },
     have h3 : (M m []).fst  = (N m []).fst,
     { by_cases h4 : k = m,
       { subst h4, apply h0.right },
       rw h0.left _ (ne.symm h4) },
-    simp only [term.val, h2, h3]
+    simp only [term₂.val, h2, h3]
   end
 | (a & (b & c)) h1 :=
   begin
@@ -146,29 +173,29 @@ lemma val_eq_val_of_eq_except {M N : model α} {k : nat} (h0 : eq_except M N k) 
     { apply val_eq_val_of_eq_except a h1.left },
     have h3 : (b & c).val M = (b & c).val N,
     { apply val_eq_val_of_eq_except (b & c) h1.right },
-    simp only [term.val, h2, h3]
+    simp only [term₂.val, h2, h3]
   end
 
 lemma holds_iff_holds_of_eq_except :
-  ∀ {M N : model α} {k : nat} (p : form),
+  ∀ {M N : model α} {k : nat} (p : form₂),
   eq_except M N k → p.fov k → (M ⊨ p ↔ N ⊨ p)
 | M N k ⟪b, a⟫ h0 h1 :=
   by cases b; simp [holds, val_eq_val_of_eq_except h0 a h1]
-| M N k (form.bin b p q) h0 h1 :=
+| M N k (form₂.bin b p q) h0 h1 :=
   begin
     cases h1,
-    apply holds_bin_iff_holds_bin;
+    apply form₂.holds_bin_iff_holds_bin;
     apply holds_iff_holds_of_eq_except;
     assumption
   end
-| M N k (form.qua b p)   h0 h1 :=
+| M N k (form₂.qua b p)   h0 h1 :=
   begin
     apply holds_qua_iff_holds_qua, intro v,
     apply holds_iff_holds_of_eq_except _
       (assign_eq_except_assign _ h0) h1
   end
 
-def ex_fa_swap_eqv [inhabited α] (p : form) :
+def ex_fa_swap_eqv [inhabited α] (p : form₂) :
   p.fov 1 → (∃* (∀* $ p.swap 0) <==α==> ∀* (∃* p)) :=
 begin
   intros h0 M,
@@ -190,10 +217,10 @@ begin
   apply (denote_evaluate (vᵈ))
 end
 
-lemma neg_swap {p : form} : (p.swap 0).neg <==α==> p.neg.swap 0 :=
+lemma neg_swap {p : form₂} : (p.swap 0).neg <==α==> p.neg.swap 0 :=
 neg_subst _ _
 
-def fa_ex_swap_eqv [inhabited α] (p : form) :
+def fa_ex_swap_eqv [inhabited α] (p : form₂) :
   p.fov 1 → (∀* (∃* $ p.swap 0) <==α==> ∃* (∀* p)) :=
 begin
   intro h0,
@@ -203,82 +230,134 @@ begin
     (qua_eqv_qua (qua_eqv_qua neg_swap))
     (@ex_fa_swap_eqv α _ _ h0),
   rw ← neg_eqv_neg,
-  simp only [holds_neg.symm, form.neg, bnot, h1]
+  simp only [holds_neg.symm, form₂.neg, bnot, h1]
 end
 
-def swap_eqv [inhabited α] (ae : bool) {p : form} :
+def swap_eqv [inhabited α] (ae : bool) {p : form₂} :
   p.fov 1 →
-  (form.qua ae (form.qua (bnot ae) $ p.swap 0)
-    <==α==> form.qua (bnot ae) (form.qua ae p)) :=
+  (form₂.qua ae (form₂.qua (bnot ae) $ p.swap 0)
+    <==α==> form₂.qua (bnot ae) (form₂.qua ae p)) :=
 by { intro h0, cases ae,
      exact fa_ex_swap_eqv _ h0,
      exact ex_fa_swap_eqv _ h0 }
 
-lemma fov_swap_zero_aux :
-  ∀ k : nat, ∀ p : form, p.fov (k + 1) → (p.swap k).fov k
-| k ⟪b, a⟫           h0 := fov_succ _ _ h0
-| k (form.bin b p q) h0 :=
-  by { cases h0, constructor;
-       apply fov_swap_zero_aux; assumption }
-| k (form.qua b p)   h0 := fov_swap_zero_aux (k + 1) p h0
+namespace form₂
 
-lemma fov_swap_zero {p : form} :
-  p.fov 1 → (p.swap 0).fov 0 :=
-fov_swap_zero_aux 0 _
+open nat
 
 lemma fov_swap :
-  ∀ k m : nat, m + 1 < k →
-  ∀ p : form, p.fov k → (p.swap m).fov k
-| k m h0 ⟪b, a⟫           h1 := fov_succ_succ _ _ h0 _ h1
-| k m h0 (form.bin b p q) h1 :=
-  by { cases h1, constructor;
+  ∀ {k : nat} {p : form₂}, p.fov (k + 1) → (p.swap k).fov k
+| k ⟪b, a⟫           h0 := term₂.fov_swap _ _ h0
+| k (form₂.bin b p q) h0 :=
+  by { cases h0, constructor;
        apply fov_swap; assumption }
-| k m h0 (form.qua b p)   h1 :=
-  fov_swap (k + 1) (m + 1) (succ_lt_succ h0) p h1
+| k (form₂.qua b p)   h0 := @fov_swap (k + 1) p h0
 
-def swap_many (ae : bool) : form → form
-| (form.qua b p) :=
-  have form.size_of (p.swap 0) < form.size_of (form.qua b p),
-  { unfold form.swap, rw form.size_of_subst,
-    simp only [form.size_of, nat.lt_succ_self, add_comm] },
+lemma fov_swap_of_ne :
+  ∀ k m : nat, (k ≠ m) → (k ≠ m + 1) →
+  ∀ p : form₂, p.fov k → (p.swap m).fov k
+| k m hO hS ⟪b, a⟫ h1 := term₂.fov_swap_of_ne hO hS _ h1
+| k m hO hS (form₂.bin b p q) h1 :=
+  by { cases h1, constructor;
+       apply fov_swap_of_ne; assumption }
+| k m hO hS (form₂.qua b p)   h1 :=
+  fov_swap_of_ne (k + 1) (m + 1)
+    (succ_ne_succ hO) (succ_ne_succ hS) p h1
+
+end form₂
+--lemma fov_swap_zero {p : form₂} :
+--  p.fov 1 → (p.swap 0).fov 0 :=
+--fov_swap_zero_aux 0 _
+
+--lemma fov_swap :
+--  ∀ k m : nat, m + 1 < k →
+--  ∀ p : form₂, p.fov k → (p.swap m).fov k
+--| k m h0 ⟪b, a⟫           h1 := fov_succ_succ _ _ h0 _ h1
+--| k m h0 (form₂.bin b p q) h1 :=
+--  by { cases h1, constructor;
+--       apply fov_swap; assumption }
+--| k m h0 (form₂.qua b p)   h1 :=
+--  fov_swap (k + 1) (m + 1) (succ_lt_succ h0) p h1
+
+lemma foq_swap (b : bool) :
+  ∀ (k : nat) {p : form₂}, foq b p → foq b (p.swap k)
+| k ⟪_, a⟫           h0 := trivial
+| k (form₂.bin _ p q) h0 := ⟨foq_swap _ h0.left, foq_swap _ h0.right⟩
+| k (form₂.qua c p)   h0 :=
+  begin
+    constructor,
+    { intro h1,
+      apply form₂.fov_swap_of_ne 0 (k + 1)
+        (zero_ne_succ _) (zero_ne_succ _) p (h0.left h1) },
+    apply foq_swap _ h0.right
+  end
+
+def swap_many (ae : bool) : form₂ → form₂
+| (form₂.qua b p) :=
+  have form₂.size_of (p.swap 0) < form₂.size_of (form₂.qua b p),
+  { unfold form₂.swap, rw form₂.size_of_subst,
+    simp only [form₂.size_of, nat.lt_succ_self, add_comm] },
   if ae = b
-  then form.qua ae (swap_many $ p.swap 0)
-  else form.qua (bnot ae) (form.qua b p)
-| p := form.qua (bnot ae) p
+  then form₂.qua ae (swap_many $ p.swap 0)
+  else form₂.qua (bnot ae) (form₂.qua b p)
+| p := form₂.qua (bnot ae) p
 
 lemma fov_swap_many (ae : bool) :
-  ∀ {p : form} {k : nat},
+  ∀ {p : form₂} {k : nat},
   p.fov (k + 1) → (swap_many ae p).fov k
 | ⟪b, a⟫           := λ _, id
-| (form.bin b p q) := λ _, id
-| (form.qua b p)   :=
-  have form.size_of (p.swap 0) < form.size_of (form.qua b p),
-  by { unfold form.swap,
-       rw form.size_of_subst,
-       form.show_size_lt},
+| (form₂.bin b p q) := λ _, id
+| (form₂.qua b p)   :=
+  have form₂.size_of (p.swap 0) < form₂.size_of (form₂.qua b p),
+  by { unfold form₂.swap,
+       rw form₂.size_of_subst,
+       form₂.show_size_lt},
   begin
     intros k h0,
     unfold swap_many,
     by_cases h1 : ae = b,
     { subst h1, rw if_pos rfl,
       have h2 : (p.swap 0).fov (k + 2) :=
-      @fov_swap (k + 2) 0
-        (succ_lt_succ $ zero_lt_succ _) _ h0,
-      apply @fov_swap_many _ (k + 1) h2 },
+      @form₂.fov_swap_of_ne (k + 2) 0 (zero_ne_succ _).symm
+        (succ_ne_succ (zero_ne_succ _).symm) _ h0,
+    apply @fov_swap_many _ (k + 1) h2 },
     rw if_neg h1, exact h0
   end
 
+lemma bnot_ne_self (b : bool) :
+  bnot b ≠ b := by { cases b; rintro ⟨_⟩ }
+
+lemma foq_swap_many (b : bool) :
+  ∀ {p : form₂}, p.fov 0 → foq b p → foq b (swap_many (bnot b) p)
+| (form₂.lit b a)   h0 h1 := ⟨λ _, h0, h1⟩
+| (form₂.bin b p q) h0 h1 := ⟨λ _, h0, h1⟩
+| (form₂.qua c p)   h0 h1 :=
+  have form₂.size_of (form₂.swap 0 p) <
+       form₂.size_of (form₂.qua c p),
+  { unfold form₂.swap, rw form₂.size_of_subst, form₂.show_size_lt },
+  begin
+    unfold swap_many,
+    by_cases h2 : bnot b = c,
+    { rw if_pos h2,
+      refine ⟨λ h3, absurd h3.symm (bnot_ne_self b), _⟩,
+      apply @foq_swap_many (p.swap 0),
+      apply form₂.fov_swap h0,
+      apply foq_swap _ _ h1.right },
+    rw if_neg h2,
+    refine ⟨λ _, h0, h1⟩
+  end
+
 lemma swap_many_eqv (α : Type u) [inhabited α] (ae : bool) :
-  ∀ {p : form}, p.fov 0 →
-  (swap_many ae p <==α==> form.qua (bnot ae) p)
+  ∀ {p : form₂}, p.fov 0 →
+  (swap_many ae p <==α==> form₂.qua (bnot ae) p)
 | ⟪b, a⟫           := λ _, eqv_refl _ _
-| (form.bin b p q) := λ _, eqv_refl _ _
-| (form.qua b p)   :=
-  have form.size_of (p.swap 0) <
-       form.size_of (form.qua b p) :=
-  by { unfold form.swap,
-       rw form.size_of_subst,
-       form.show_size_lt },
+| (form₂.bin b p q) := λ _, eqv_refl _ _
+| (form₂.qua b p)   :=
+  have form₂.size_of (p.swap 0) <
+       form₂.size_of (form₂.qua b p) :=
+  by { unfold form₂.swap,
+       rw form₂.size_of_subst,
+       form₂.show_size_lt },
   begin
     intro h0,
     unfold swap_many,
@@ -287,27 +366,27 @@ lemma swap_many_eqv (α : Type u) [inhabited α] (ae : bool) :
       apply eqv_trans _ (@swap_eqv α _ ae _ h0),
       apply qua_eqv_qua,
       apply swap_many_eqv,
-      apply fov_swap_zero,
+      apply form₂.fov_swap,
       apply h0 },
     rw if_neg h1, apply eqv_refl _
   end
 
-def swap_all (ae : bool) : form → form
+def swap_all (ae : bool) : form₂ → form₂
 | ⟪b, a⟫           := ⟪b, a⟫
-| (form.bin b p q) :=
+| (form₂.bin b p q) :=
   pull (some ae) b tt (swap_all p) (swap_all q)
-| (form.qua b p)   :=
+| (form₂.qua b p)   :=
   if ae = b
-  then form.qua ae (swap_all p)
+  then form₂.qua ae (swap_all p)
   else swap_many ae (swap_all p)
 
 lemma fov_swap_all (ae : bool) :
-  ∀ {k : nat} {p : form}, p.fov k → (swap_all ae p).fov k
+  ∀ {k : nat} {p : form₂}, p.fov k → (swap_all ae p).fov k
 | k ⟪b, a⟫           h0 := h0
-| k (form.bin b p q) h0 :=
+| k (form₂.bin b p q) h0 :=
   by { cases h0, apply fov_pull;
        apply fov_swap_all; assumption }
-| k (form.qua b p)   h0 :=
+| k (form₂.qua b p)   h0 :=
   begin
     unfold swap_all,
     by_cases h1 : ae = b,
@@ -319,16 +398,41 @@ lemma fov_swap_all (ae : bool) :
     apply h0
   end
 
+lemma foq_swap_all (b : bool) :
+  ∀ {p : form₂}, (foq b p) → foq b (swap_all (bnot b) p)
+| ⟪_, a⟫           h0 := trivial
+| (form₂.bin _ p q) h0 :=
+  begin
+    unfold swap_all,
+    have hp := foq_swap_all h0.left,
+    have hq := foq_swap_all h0.right,
+    apply foq_pull; assumption
+  end
+| (form₂.qua c p) h0 :=
+  begin
+    unfold swap_all,
+    by_cases h1 : (bnot b = c),
+    { rw if_pos h1,
+      refine ⟨ λ h2, absurd h2.symm (bnot_ne_self b),
+               foq_swap_all h0.right ⟩ },
+    rw if_neg h1,
+    have h2 : (swap_all (bnot b) p).fov 0,
+    { apply fov_swap_all,
+      apply h0.left _,
+      rwa [bnot_eq_iff_ne, not_not] at h1 },
+    apply foq_swap_many _ h2 (foq_swap_all h0.right)
+  end
+
 lemma swap_all_eqv [inhabited α] {ae : bool} :
-  ∀ {p : form}, foq (bnot ae) p → (swap_all ae p <==α==> p)
+  ∀ {p : form₂}, foq (bnot ae) p → (swap_all ae p <==α==> p)
 | ⟪b, a⟫           h0 := eqv_refl _ _
-| (form.bin b p q) h0 :=
+| (form₂.bin b p q) h0 :=
   eqv_trans
     (pull_eqv ae b _ _ _)
     (bin_eqv_bin
       (swap_all_eqv h0.left)
       (swap_all_eqv h0.right))
-| (form.qua b p)   h0 :=
+| (form₂.qua b p)   h0 :=
   begin
     unfold swap_all,
     by_cases h1 : ae = b,
@@ -341,44 +445,212 @@ lemma swap_all_eqv [inhabited α] {ae : bool} :
     apply qua_eqv_qua (swap_all_eqv h0.right)
 end
 
-def prenexify : form → form
+def prenexify : form₂ → form₂
 | ⟪b, a⟫           := ⟪b, a⟫
-| (form.bin b p q) :=
+| (form₂.bin b p q) :=
   pull none b tt (prenexify p) (prenexify q)
-| (form.qua b p)   := form.qua b (prenexify p)
+| (form₂.qua b p)   := form₂.qua b (prenexify p)
+
+lemma fov_prenexify :
+  ∀ {k : nat} {p : form₂}, p.fov k → (prenexify p).fov k
+| k ⟪_, a⟫           h0 := h0
+| k (form₂.bin _ p q) h0 :=
+  by { cases h0, apply fov_pull;
+       apply fov_prenexify; assumption }
+| k (form₂.qua c p)   h0 := @fov_prenexify (k + 1) p h0
+
+lemma foq_prenexify (b : bool) :
+  ∀ {p : form₂}, (foq b p) → foq b (prenexify p)
+| ⟪_, a⟫           h0 := h0
+| (form₂.bin _ p q) h0 :=
+  by { cases h0, apply foq_pull;
+       apply foq_prenexify; assumption }
+| (form₂.qua c p)   h0 :=
+  ⟨ λ h1, fov_prenexify (h0.left h1),
+    foq_prenexify h0.right ⟩
 
 lemma prenexify_eqv [inhabited α] :
-  ∀ p : form, prenexify p <==α==> p
+  ∀ p : form₂, prenexify p <==α==> p
 | ⟪b, a⟫           := eqv_refl _ _
-| (form.bin b p q) :=
+| (form₂.bin b p q) :=
   begin
     apply eqv_trans (@pull_eqv α _ _ _ _ _ _),
     apply bin_eqv_bin;
     apply prenexify_eqv
   end
-| (form.qua b p)   := qua_eqv_qua (prenexify_eqv _)
+| (form₂.qua b p)   := qua_eqv_qua (prenexify_eqv _)
 
-def AE : form → form := prenexify ∘ swap_all ff
+def QDFy (b : bool) : form₂ → form₂ := prenexify ∘ swap_all b
 
-lemma AE_eqv [inhabited α] (p : form) :
-  foq tt p → (AE p <==α==> p) :=
-λ h, eqv_trans (prenexify_eqv _) (swap_all_eqv h)
+lemma N_subst {b : bool} :
+  ∀ {p : form₂} (σ : sub₂), p.N b → (p.subst σ).N b
+| ⟪_, a⟫           _ _ := trivial
+| (form₂.bin c p q) _ h := ⟨N_subst _ h.left, N_subst _ h.right⟩
+| (form₂.qua c p)   σ h := ⟨h.left, N_subst _ h.right⟩
 
-def EA : form → form := prenexify ∘ swap_all tt
+lemma QN_subst {b : bool} :
+  ∀ {p : form₂} (σ : sub₂), p.QN b → (p.subst σ).QN b
+| ⟪_, a⟫           _ h0 := trivial
+| (form₂.bin c p q) _ h0 :=
+  by { cases h0, constructor;
+       apply N_subst; assumption }
+| (form₂.qua c p)   σ h0 :=
+  ⟨ λ h1, QN_subst _ (h0.left h1),
+    λ h1, N_subst _ (h0.right h1) ⟩
 
-lemma EA_eqv [inhabited α] (p : form) :
-  foq ff p → (EA p <==α==> p) :=
-λ h, eqv_trans (prenexify_eqv _) (swap_all_eqv h)
+lemma QN_swap_many {b : bool} :
+  ∀ {p : form₂}, p.QN b → (swap_many b p).QN b
+| (form₂.lit c a) :=
+  λ h0, ⟨ λ h1, absurd h1 (bnot_ne_self b).symm, λ _, h0⟩
+| (form₂.bin c p q) :=
+  λ h0, ⟨ λ h1, absurd h1 (bnot_ne_self b).symm, λ _, h0⟩
+| (form₂.qua c p) :=
+  have form₂.size_of (form₂.swap 0 p) <
+       form₂.size_of (form₂.qua c p),
+  by { unfold form₂.swap,
+       rw form₂.size_of_subst,
+       form₂.show_size_lt },
+  begin
+    intro h0, unfold swap_many,
+    by_cases h1 : b = c,
+    { rw if_pos h1,
+      constructor; intro h2,
+      { apply QN_swap_many,
+        apply QN_subst _ (h0.left h1) },
+      cases h2 rfl },
+    rw if_neg h1,
+    constructor; intro h2,
+    { rw eq_bnot_iff_ne at h2,
+      cases h2 rfl },
+    refine ⟨h1, h0.right h1⟩
+  end
 
-def is_QF : form → Prop
+lemma QN_swap_all (b : bool) :
+  ∀ p : form₂, (swap_all b p).QN b
+| ⟪_, a⟫           := trivial
+| (form₂.bin c p q) :=
+  by { unfold swap_all, apply QN_pull; apply QN_swap_all }
+| (form₂.qua c p)   :=
+  begin
+    unfold swap_all,
+    by_cases h0 : b = c,
+    { rw if_pos h0,
+      constructor; intro h1,
+      { apply QN_swap_all },
+      cases (h1 rfl) },
+    rw if_neg h0,
+    have h1 := QN_swap_all p,
+    apply QN_swap_many h1
+  end
+
+lemma QF_prenexify {b : bool} :
+  ∀ {p : form₂}, p.N b → (prenexify p).QF (bnot b)
+| (form₂.lit c a)   h0 := trivial
+| (form₂.bin c p q) h0 :=
+  by { cases h0,  apply QF_pull;
+       apply QF_prenexify; assumption }
+| (form₂.qua c p)   h0 :=
+  by { constructor,
+       { rw bnot_eq_iff_ne, apply h0.left },
+       apply QF_prenexify h0.right }
+
+lemma QDF_prenexify (b : bool) :
+  ∀ p : form₂, p.QN b → (prenexify p).QDF b
+| (form₂.lit c a)   h0 := trivial
+| (form₂.qua c p)   h0 :=
+  begin
+    by_cases h1 : b = c,
+    { constructor; intro h2,
+      { apply QDF_prenexify _ (h0.left h1) },
+      cases h2 h1 },
+    constructor; intro h2,
+    { cases h1 h2 },
+    apply QF_prenexify (h0.right h2)
+  end
+| (form₂.bin c p q) h0 :=
+  by { cases h0, apply form₂.QDF_of_QF_bnot,
+       apply QF_pull; apply QF_prenexify; assumption }
+
+lemma QDF_QDFy (b : bool) (p : form₂) : (QDFy b p).QDF b :=
+by {apply QDF_prenexify, apply QN_swap_all}
+
+
+#exit
+
+lemma in_blocks (b : bool) : form₂ → Prop
+
+
+
+end form₂
+
+
+#exit
+
+def is_AE : form₂ → Prop
+| (∀* p) := is_AE p
+| p      := is_E p
+def AE : form₂ → form₂ := prenexify ∘ swap_all ff
+
+def is_AF : form₂ → Prop
 | ⟪_, _⟫           := true
-| (form.bin _ p q) := is_QF p ∧ is_QF q
-| (form.qua b p)   := false
+| (form₂.bin _ p q) := is_AF p ∧ is_AF q
+| (∀* p)           := false
+| (∃* p)           := is_AF p
 
-def is_E : form → Prop
+def is_AAF : form₂ → Prop
+| (∀* p) := is_AAF p
+| p      := is_AF p
+
+
+
+lemma is_AAF_swap_all_ff :
+  ∀ p : form₂, is_AAF (swap_all ff p)
+| ⟪_, _⟫           := true
+| (form₂.bin _ p q) :=
+  ⟨ is_AAF_swap_all_ff _,
+    is_AAF_swap_all_ff _ ⟩
+
+ #exit
+--| (∀* p)           := --false
+| (∃* p)           := --is_AF p
+
+#exit
+lemma foex_AE (p : form₂) :
+  foq tt p → foq tt (AE p) :=
+λ h, foq_prenexify _ (foq_swap_all _ h)
+
+
+
+def is_E : form₂ → Prop
 | (∃* p) := is_E p
 | p      := is_QF p
 
-def is_AE : form → Prop
+def is_AE : form₂ → Prop
 | (∀* p) := is_AE p
 | p      := is_E p
+
+
+
+#exit
+lemma is_AE_AE (p : form₂) : is_AE (AE p) := sorry
+
+
+
+#exit
+
+lemma AE_eqv [inhabited α] (p : form₂) :
+  foq tt p → (AE p <==α==> p) :=
+λ h, eqv_trans (prenexify_eqv _) (swap_all_eqv h)
+
+#exit
+def EA : form₂ → form₂ := prenexify ∘ swap_all tt
+
+
+
+
+
+
+
+lemma EA_eqv [inhabited α] (p : form₂) :
+  foq ff p → (EA p <==α==> p) :=
+λ h, eqv_trans (prenexify_eqv _) (swap_all_eqv h)
