src/tactic/fol/term.lean
@@ -1,64 +1,97 @@
-import .model .misc tactic.interactive
+import .nat .model
 
-universe u 
+universe u
 
 variable {α : Type u}
 
-local notation f `₀↦` a := assign a f
-
 @[derive has_reflect, derive decidable_eq]
 inductive term : Type
-| var : nat → term
+| sym : nat  → term
 | app : term → term → term
+| vpp : term → nat  → term
 
-local notation `#` := term.var
+local notation `&`     := term.sym
 local notation a `&` b := term.app a b
+local notation a `#` k := term.vpp a k
 
 namespace term
 
-def incr_idxs_ge (k : nat) : term → term
-| (# m)   := if k ≤ m then # (m + 1) else # m
-| (a & b) := a.incr_idxs_ge & b.incr_idxs_ge  
+def repr_core : bool → term → string
+| s (term.sym k)   := (if s then "P" else "F") ++ k.to_subs
+| s (term.app a b) := "(" ++ a.repr_core s ++ " " ++ b.repr_core ff ++ ")"
+| s (term.vpp a k) := "(" ++ a.repr_core s ++ " " ++ "X" ++ k.to_subs ++ ")"
 
-def incr_idxs : term → term := incr_idxs_ge 0
+def repr : term → string := repr_core tt
 
-def val (M : model α) : term → value α
-| (# k)   := M k
-| (a & b) := a.val ∘ list.cons (b.val []).fst
+def vdxs : term → list nat
+| (term.sym _)   := []
+| (term.app a b) := a.vdxs ∪ b.vdxs
+| (term.vpp a m) := a.vdxs.insert m
 
-end term 
-
-lemma incr_idxs_app (a b : term) : 
-  term.incr_idxs (a & b) = (a.incr_idxs & b.incr_idxs) := 
-by simp only [ term.incr_idxs, and_self,
-     term.incr_idxs_ge, eq_self_iff_true ]
-
-namespace term
-
-lemma val_assign_incr_idxs (M : model α) (v : value α) :
-  ∀ a : term, val (M ₀↦ v) a.incr_idxs = val M a 
-| (# k)   := rfl
-| (a & b) := 
-  by simp only [val, val_assign_incr_idxs a, 
-     val_assign_incr_idxs b, incr_idxs_app]
+def val (M : model α) (v : nat → α) : term → value α
+| (term.sym k)   := M k
+| (term.app a b) := a.val ∘ list.cons (b.val []).fst
+| (term.vpp a k) := a.val ∘ list.cons (v k)
 
 end term
 
-lemma eq_of_var_eq_var {k m : nat} : (# k) = (# m) → k = m :=
-by {intro h0, cases h0, refl}
+def sub : Type := list (nat × term)
 
-lemma val_incr_idxs_ge {M N : model α} {k : nat}  
-  (h0 : ∀ m < k, M m = N m) (h1 : ∀ m ≥ k, M (m + 1) = N m) : 
-    ∀ a : term, (a.incr_idxs_ge k).val M = a.val N 
-| (# m) := 
-  begin
-    unfold term.incr_idxs_ge,
-    by_cases h2 : k ≤ m,
-    { rw if_pos h2, 
-      apply h1 _ h2 },
-    rw if_neg h2,
-    rw not_le at h2,
-    apply h0 _ h2
+def sub.get (σ : sub) (k : nat) : option term :=
+prod.snd <$> (list.find (eq k ∘ prod.fst)) σ
+
+namespace vas
+
+def subst (M : model α) (v : vas α) (σ : sub) (k : nat) : α :=
+match σ.get k with
+| none   := v k
+| some t := (t.val M v []).fst
+end
+
+lemma subst_eq_of_eq_none (M : model α)
+  (v : vas α) {σ : sub} {k : nat} :
+σ.get k = none → v.subst M σ k = v k :=
+by { intro h1, simp only [h1, subst] }
+
+lemma subst_eq_of_eq_some (M : model α)
+  (v : vas α) {σ : sub} {k : nat} {t : term} :
+σ.get k = some t → v.subst M σ k = (t.val M v []).fst :=
+by { intro h1, simp only [h1, subst] }
+
+end vas
+
+namespace term
+
+def subst (σ : sub) : term → term
+| (& k)   := & k
+| (t & s) := subst t & subst s
+| (t # k) :=
+  match σ.get k with
+  | none   := subst t # k
+  | some s := subst t & s
   end
-| (a & b) := 
-  by simp only [term.incr_idxs_ge, term.val, val_incr_idxs_ge]
+
+lemma subst_eq_of_eq_none {σ : sub} (t : term) {k : nat} :
+σ.get k = none → subst σ (t # k) = subst σ t # k :=
+by { intro h, simp only [h, subst, eq_self_iff_true, and_self] }
+
+lemma subst_eq_of_eq_some {σ : sub} (t s : term) {k : nat} :
+σ.get k = some s → subst σ (t # k) = (subst σ t & s) :=
+by { intro h, simp only [h, subst, eq_self_iff_true, and_self] }
+
+lemma val_subst (M : model α) (v : vas α) (σ : sub) :
+  ∀ t : term, (t.subst σ).val M v = t.val M (v.subst M σ)
+| (& k)   := rfl
+| (t & s) := by simp only [val, subst, val_subst]
+| (t # k) := --by simp only [val, subst, val_subst]
+  begin
+    cases h1 : σ.get k with s,
+    simp only [subst_eq_of_eq_none t h1,
+      vas.subst_eq_of_eq_none M v h1,
+      val_subst, val],
+    simp only [subst_eq_of_eq_some t s h1,
+      vas.subst_eq_of_eq_some M v h1,
+      val_subst, val]
+  end
+
+end term
